Update Map.dfy

Map.dfy
@@ -5,7 +5,7 @@
 
   Project 3 -- Part A
 
-  Your name(s): 
+  Your name(s): Mitchell Piehl and Josh Bergthold
   ===============================================*/
 
 include "Option.dfy"
@@ -42,20 +42,30 @@ module Map {
   // every key in m has exactly one associated value (no contract needed) 
   ghost predicate isValid<T(!new)>(m: Map<T>)
   {
-    true // replace this line with your definition
+  match m
+  case Nil => true
+  case Cons(e, Nil) =>
+    true
+  case Cons((k,_), t) =>
+    isValid(t) && k !in keys(t)
   }
 
   // For every value type T, emptyMap<T>() is 
   // the empty map of elements of type T
   function emptyMap<T(!new)>(): Map<T> 
+    ensures isValid(emptyMap<T>())
   { Nil }
 
   // isEmpty(m) is true iff m has no entries 
   predicate isEmpty<T(!new)>(m: Map<T>)
+    ensures m == Nil <==> isEmpty(m)
   { m == Nil }
 
   // size(m) is the number of entries in m
   function size<T(==,!new)>(m: Map<T>): nat 
+    requires isValid(m)
+    ensures isEmpty(m) <==> size(m) == 0
+    ensures !isEmpty(m) ==> size(m) > 0
   {
     match m
     case Nil => 0
@@ -64,6 +74,8 @@ module Map {
 
   // keys(m) is the set of keys in m's entries
   function keys<T(!new)>(m: Map<T>): set<int>
+    decreases m
+    ensures isEmpty(m) <==> keys(m) == {}
   {
     match m
     case Nil => {}
@@ -72,6 +84,13 @@ module Map {
 
   // values(m) is the set of values in m's entries
   function values<T(!new)>(m: Map<T>): set<T>
+    requires isValid(m)
+    ensures isValid(m)
+
+    ensures isEmpty(m) <==> values(m) == {}
+    ensures |values(m)| <= size(m)
+
+    ensures forall i: int :: (get(m, i) != None) <==> i in keys(m)
   {
     match m
     case Nil => {}
@@ -82,6 +101,10 @@ module Map {
   // More precisely, it is Some(v) if k has an associated value v,
   // and is None otherwhise.
   function get<T(!new)>(m: Map<T>, k: int): Option<T>
+    requires isValid(m)
+    ensures isValid(m)
+    ensures (get(m,k) == None) <==> k !in keys(m)
+    ensures (get(m,k) != None) ==> (k, (get(m,k)).val) in entries(m)
   {
     match m
     case Nil => None
@@ -95,6 +118,16 @@ module Map {
   // remove(m, k) is the map obtained from m by removing from it
   // the entry with key k, if any.
   function remove<T(!new)>(m: Map<T>, k: int): Map<T>
+    requires isValid(m)
+    ensures isValid(remove(m,k))
+
+    ensures keys(remove(m,k)) == keys(m) - {k}
+    ensures get(remove(m,k), k) == None
+    ensures forall q: int :: q != k ==> get(remove(m,k), q) == get(m,q)
+
+    ensures k !in keys(m) ==> size(remove(m,k)) == size(m) 
+    ensures k in keys(m) ==> size(remove(m,k)) == size(m) -1
+    ensures values(remove(m,k)) <= values(m)
   {
     match m
     case Nil => Nil
@@ -109,6 +142,19 @@ module Map {
   // put(m, k, v) is the map that associates key k with value v
   // and is othewise identical to m.
   function put<T(!new)>(m: Map<T>, k: int, v: T): Map<T>
+    requires isValid(m)
+    ensures isValid(put(m,k,v))
+
+    ensures keys(put(m,k,v)) == keys(m) + {k}
+    ensures v in values(put(m, k, v))
+    ensures (k, v) in entries(put(m, k,v))
+
+    ensures get(put(m,k,v), k) == Some(v)
+    ensures forall q :: q != k ==> get(put(m,k,v), q) == get(m, q)
+
+    ensures k in keys(m) ==> size(put(m,k,v)) == size(m) 
+    ensures k !in keys(m) ==> size(put(m,k,v)) == size(m) + 1
+    ensures values(put(m, k, v)) <= values(m) + {v}
   {
     match m
     case Nil => Cons((k, v), Nil)
